Replace some new_recursive_definition with Definition (nocompute) (#1694)
Co-authored-by: Michael Norrish <Michael.Norrish@anu.edu.au>

src/real/analysis/polyScript.sml
@@ -108,31 +108,30 @@ QED
 (* Application of polynomial as a real function.                             *)
 (* ------------------------------------------------------------------------- *)
 
-fun new_recursive_definition ax name def =
-     Prim_rec.new_recursive_definition
-       {name=name, def=def, rec_axiom=ax};
-
-val poly = new_recursive_definition list_Axiom "poly_def"
-  (Term`(poly [] x = 0r) /\
-        (poly (h::t) x = h + x * poly t x)`);
+Definition poly_def[nocompute]:
+  (poly [] x = 0r) /\
+  (poly (h::t) x = h + x * poly t x)
+End
 
 
 (* ------------------------------------------------------------------------- *)
 (* Arithmetic operations on polynomials. Overloaded (not sure this is wise). *)
 (* ------------------------------------------------------------------------- *)
 
-val poly_add = new_recursive_definition list_Axiom "poly_add_def"
- (Term`(poly_add [] l2 = l2) /\
-       (poly_add (h::t) l2 = if (l2 = []) then h::t
-                             else  ((h:real) + HD l2)::poly_add t (TL l2))`);
+Definition poly_add_def[nocompute]:
+  (poly_add [] l2 = l2) /\
+  (poly_add (h::t) l2 = if (l2 = []) then h::t
+                        else  ((h:real) + HD l2)::poly_add t (TL l2))
+End
 
 Overload "+" = Term`poly_add`
 
 val _ = Parse.hide "##";
 
-val poly_cmul = new_recursive_definition list_Axiom "poly_cmul_def"
- (Term`($## c [] = []) /\
-       ($## c (h::t) = (c:real * h) :: ($## c t))`);
+Definition poly_cmul_def[nocompute]:
+  ($## c [] = []) /\
+  ($## c (h::t) = (c:real * h) :: ($## c t))
+End
 val _ = set_fixity "##" (Infixl 600);
 
 Definition poly_neg_def[nocompute]: poly_neg = $## (~(&1))
@@ -140,17 +139,17 @@ End
 
 Overload "~" = Term`poly_neg`
 
-val poly_mul = new_recursive_definition list_Axiom "poly_mul_def"
- (Term`(poly_mul [] l2     = []) /\
-       (poly_mul (h::t) l2 = if (t = []) then h ## l2
-                             else (h ## l2) + (0r :: poly_mul t l2))`);
+Definition poly_mul_def[nocompute]:
+  (poly_mul [] l2     = []) /\
+  (poly_mul (h::t) l2 = if (t = []) then h ## l2
+                        else (h ## l2) + (0r :: poly_mul t l2))
+End
+Overload "*" = “poly_mul”
 
-Overload "*" = Term`poly_mul`
-
-val poly_exp = new_recursive_definition num_Axiom "poly_exp_def"
- (Term`(poly_exp p 0       = [1r]) /\
-       (poly_exp p (SUC n) = poly_mul p (poly_exp p n))`);
-
+Definition poly_exp_def[nocompute]:
+  (poly_exp p 0       = [1r]) /\
+  (poly_exp p (SUC n) = poly_mul p (poly_exp p n))
+End
 val _ = set_fixity "poly_exp" (Infixr 700) ;
 
 
@@ -158,15 +157,14 @@ val _ = set_fixity "poly_exp" (Infixr 700) ;
 (* Differentiation of polynomials (needs an auxiliary function).             *)
 (* ------------------------------------------------------------------------- *)
 
-val poly_diff_aux = new_recursive_definition list_Axiom
-  "poly_diff_aux_def"
-   (Term`(poly_diff_aux n [] = []) /\
-         (poly_diff_aux n (h::t) = (&n * h) :: poly_diff_aux (SUC n) t)`);
+Definition poly_diff_aux_def[nocompute]:
+  (poly_diff_aux n [] = []) /\
+  (poly_diff_aux n (h::t) = (&n * h) :: poly_diff_aux (SUC n) t)
+End
 
 Definition poly_diff_def[nocompute]:
   diff l = if l = [] then [] else poly_diff_aux 1 (TL l)
 End
-
 
 (* ------------------------------------------------------------------------- *)
 (* Useful clausifications.                                                   *)
@@ -177,16 +175,16 @@ Theorem POLY_ADD_CLAUSES:
       (p1 + [] = p1) /\
    ((h1::t1) + (h2::t2) = (h1 + h2) :: (t1 + t2))
 Proof
-  REWRITE_TAC[poly_add, NOT_CONS_NIL, HD, TL] THEN
+  REWRITE_TAC[poly_add_def, NOT_CONS_NIL, HD, TL] THEN
   SPEC_TAC(Term`p1:real list`,Term`p1:real list`) THEN
-  LIST_INDUCT_TAC THEN ASM_REWRITE_TAC[poly_add]
+  LIST_INDUCT_TAC THEN ASM_REWRITE_TAC[poly_add_def]
 QED
 
 Theorem POLY_CMUL_CLAUSES:
  (c ## [] = []) /\
       (c ## (h::t) = (c * h) :: (c ## t))
 Proof
-  REWRITE_TAC[poly_cmul]
+  REWRITE_TAC[poly_cmul_def]
 QED
 
 Theorem POLY_NEG_CLAUSES:
@@ -201,7 +199,7 @@ Theorem POLY_MUL_CLAUSES:
     ([h1] * p2 = h1 ## p2) /\
    ((h1::k1::t1) * p2 = (h1 ## p2) + (&0 :: ((k1::t1) * p2)))
 Proof
-  REWRITE_TAC[poly_mul, NOT_CONS_NIL]
+  REWRITE_TAC[poly_mul_def, NOT_CONS_NIL]
 QED
 
 Theorem POLY_DIFF_CLAUSES:
@@ -209,7 +207,7 @@ Theorem POLY_DIFF_CLAUSES:
    (diff [c] = []) /\
    (diff (h::t) = poly_diff_aux 1 t)
 Proof
-  REWRITE_TAC[poly_diff_def, NOT_CONS_NIL, HD, TL, poly_diff_aux]
+  REWRITE_TAC[poly_diff_def, NOT_CONS_NIL, HD, TL, poly_diff_aux_def]
 QED
 
 (* ------------------------------------------------------------------------- *)
@@ -219,16 +217,16 @@ QED
 Theorem POLY_ADD:
  !p1 p2 x. poly (p1 + p2) x = poly p1 x + poly p2 x
 Proof
-  LIST_INDUCT_TAC THEN REWRITE_TAC[poly_add, poly, REAL_ADD_LID] THEN
+  LIST_INDUCT_TAC THEN REWRITE_TAC[poly_add_def, poly_def, REAL_ADD_LID] THEN
   LIST_INDUCT_TAC THEN
-  ASM_REWRITE_TAC[NOT_CONS_NIL, HD, TL, poly, REAL_ADD_RID] THEN
+  ASM_REWRITE_TAC[NOT_CONS_NIL, HD, TL, poly_def, REAL_ADD_RID] THEN
   REAL_ARITH_TAC
 QED
 
 Theorem POLY_CMUL:
  !p c x. poly (c ## p) x = c * poly p x
 Proof
-  LIST_INDUCT_TAC THEN ASM_REWRITE_TAC[poly, poly_cmul] THEN
+  LIST_INDUCT_TAC THEN ASM_REWRITE_TAC[poly_def, poly_cmul_def] THEN
   REAL_ARITH_TAC
 QED
 
@@ -243,21 +241,21 @@ Theorem POLY_MUL:
  !x p1 p2. poly (p1 * p2) x = poly p1 x * poly p2 x
 Proof
   GEN_TAC THEN LIST_INDUCT_TAC THEN
-  REWRITE_TAC[poly_mul, poly, REAL_MUL_LZERO, POLY_CMUL, POLY_ADD] THEN
+  REWRITE_TAC[poly_mul_def, poly_def, REAL_MUL_LZERO, POLY_CMUL, POLY_ADD] THEN
   SPEC_TAC(Term`h:real`,Term`h:real`) THEN
   SPEC_TAC(Term`t:real list`,Term`t:real list`) THEN
   LIST_INDUCT_TAC THEN
-  REWRITE_TAC[poly_mul, POLY_CMUL, POLY_ADD, poly, POLY_CMUL,
+  REWRITE_TAC[poly_mul_def, POLY_CMUL, POLY_ADD, poly_def, POLY_CMUL,
     REAL_MUL_RZERO, REAL_ADD_RID, NOT_CONS_NIL] THEN
-  ASM_REWRITE_TAC[POLY_ADD, POLY_CMUL, poly] THEN
+  ASM_REWRITE_TAC[POLY_ADD, POLY_CMUL, poly_def] THEN
   REAL_ARITH_TAC
 QED
 
 Theorem POLY_EXP:
  !p n (x:real). poly (p poly_exp n) x = (poly p x) pow n
 Proof
-  GEN_TAC THEN INDUCT_TAC THEN ASM_REWRITE_TAC[poly_exp, pow, POLY_MUL] THEN
-  REWRITE_TAC[poly] THEN REAL_ARITH_TAC
+  GEN_TAC THEN INDUCT_TAC THEN ASM_REWRITE_TAC[poly_exp_def, pow, POLY_MUL] THEN
+  REWRITE_TAC[poly_def] THEN REAL_ARITH_TAC
 QED
 
 (* ------------------------------------------------------------------------- *)
@@ -268,7 +266,7 @@ val POLY_DIFF_LEMMA = store_thm("POLY_DIFF_LEMMA",
  (Term`!l n x. ((\x. (x pow (SUC n)) * poly l x) diffl
                    ((x pow n) * poly (poly_diff_aux (SUC n) l) x))(x)`),
   LIST_INDUCT_TAC THEN
-  REWRITE_TAC[poly, poly_diff_aux, REAL_MUL_RZERO, DIFF_CONST] THEN
+  REWRITE_TAC[poly_def, poly_diff_aux_def, REAL_MUL_RZERO, DIFF_CONST] THEN
   MAP_EVERY X_GEN_TAC [(Term`n:num`), (Term`x:real`)] THEN
   REWRITE_TAC[REAL_LDISTRIB, REAL_MUL_ASSOC] THEN
   ONCE_REWRITE_TAC[GSYM(ONCE_REWRITE_RULE[REAL_MUL_SYM] (CONJUNCT2 pow))] THEN
@@ -288,7 +286,7 @@ val POLY_DIFF = store_thm("POLY_DIFF",
  (Term`!l x. ((\x. poly l x) diffl (poly (diff l) x))(x)`),
   LIST_INDUCT_TAC THEN REWRITE_TAC[POLY_DIFF_CLAUSES] THEN
   ONCE_REWRITE_TAC[SYM(ETA_CONV (Term`\x. poly l x`))] THEN
-  REWRITE_TAC[poly, DIFF_CONST] THEN
+  REWRITE_TAC[poly_def, DIFF_CONST] THEN
   MAP_EVERY X_GEN_TAC [(Term`x:real`)] THEN
   MP_TAC(SPECL [(Term`t:real list`), (Term`0:num`), (Term`x:real`)]
          POLY_DIFF_LEMMA) THEN
@@ -358,7 +356,7 @@ val POLY_MVT = store_thm("POLY_MVT",
 
 val POLY_ADD_RZERO = store_thm("POLY_ADD_RZERO",
  (Term`!p. poly (p + []) = poly p`),
-  REWRITE_TAC[FUN_EQ_THM, POLY_ADD, poly, REAL_ADD_RID]);
+  REWRITE_TAC[FUN_EQ_THM, POLY_ADD, poly_def, REAL_ADD_RID]);
 
 val POLY_MUL_ASSOC = store_thm("POLY_MUL_ASSOC",
  (Term`!p q r. poly (p * (q * r)) = poly ((p * q) * r)`),
@@ -367,7 +365,7 @@ val POLY_MUL_ASSOC = store_thm("POLY_MUL_ASSOC",
 val POLY_EXP_ADD = store_thm("POLY_EXP_ADD",
  (Term`!d n p. poly(p poly_exp (n + d)) = poly(p poly_exp n * p poly_exp d)`),
   REWRITE_TAC[FUN_EQ_THM, POLY_MUL] THEN
-  INDUCT_TAC THEN ASM_REWRITE_TAC[POLY_MUL, ADD_CLAUSES, poly_exp, poly] THEN
+  INDUCT_TAC THEN ASM_REWRITE_TAC[POLY_MUL, ADD_CLAUSES, poly_exp_def, poly_def] THEN
   REAL_ARITH_TAC);
 
 (* ------------------------------------------------------------------------- *)
@@ -377,15 +375,15 @@ val POLY_EXP_ADD = store_thm("POLY_EXP_ADD",
 val POLY_DIFF_AUX_ADD = store_thm("POLY_DIFF_AUX_ADD",
 (Term`!p1 p2 n. poly (poly_diff_aux n (p1 + p2)) =
              poly (poly_diff_aux n p1 + poly_diff_aux n p2)`),
-  REPEAT(LIST_INDUCT_TAC THEN REWRITE_TAC[poly_diff_aux, poly_add]) THEN
-  ASM_REWRITE_TAC[poly_diff_aux, FUN_EQ_THM, poly, NOT_CONS_NIL, HD, TL] THEN
+  REPEAT(LIST_INDUCT_TAC THEN REWRITE_TAC[poly_diff_aux_def, poly_add_def]) THEN
+  ASM_REWRITE_TAC[poly_diff_aux_def, FUN_EQ_THM, poly_def, NOT_CONS_NIL, HD, TL] THEN
   REAL_ARITH_TAC);
 
 val POLY_DIFF_AUX_CMUL = store_thm("POLY_DIFF_AUX_CMUL",
  (Term`!p c n. poly (poly_diff_aux n (c ## p)) =
            poly (c ## poly_diff_aux n p)`),
   LIST_INDUCT_TAC THEN
-  ASM_SIMP_TAC real_ac_ss [FUN_EQ_THM, poly, poly_diff_aux, poly_cmul]);
+  ASM_SIMP_TAC real_ac_ss [FUN_EQ_THM, poly_def, poly_diff_aux_def, poly_cmul_def]);
 
 val POLY_DIFF_AUX_NEG = store_thm("POLY_DIFF_AUX_NEG",
  (Term`!p n.  poly (poly_diff_aux n (poly_neg p)) =
@@ -394,8 +392,8 @@ val POLY_DIFF_AUX_NEG = store_thm("POLY_DIFF_AUX_NEG",
 
 val POLY_DIFF_AUX_MUL_LEMMA = store_thm("POLY_DIFF_AUX_MUL_LEMMA",
  (Term`!p n. poly (poly_diff_aux (SUC n) p) = poly (poly_diff_aux n p + p)`),
-  LIST_INDUCT_TAC THEN REWRITE_TAC[poly_diff_aux, poly_add, NOT_CONS_NIL] THEN
-  ASM_REWRITE_TAC[HD, TL, poly, FUN_EQ_THM] THEN
+  LIST_INDUCT_TAC THEN REWRITE_TAC[poly_diff_aux_def, poly_add_def, NOT_CONS_NIL] THEN
+  ASM_REWRITE_TAC[HD, TL, poly_def, FUN_EQ_THM] THEN
   REWRITE_TAC[GSYM REAL_OF_NUM_SUC, REAL_ADD_RDISTRIB, REAL_MUL_LID]);
 
 (* ------------------------------------------------------------------------- *)
@@ -406,12 +404,12 @@ val POLY_DIFF_ADD = store_thm("POLY_DIFF_ADD",
  (Term`!p1 p2. poly (diff (p1 + p2)) =
            poly (diff p1  + diff p2)`),
   REPEAT LIST_INDUCT_TAC THEN
-  REWRITE_TAC[poly_add, poly_diff_def, NOT_CONS_NIL, POLY_ADD_RZERO] THEN
+  REWRITE_TAC[poly_add_def, poly_diff_def, NOT_CONS_NIL, POLY_ADD_RZERO] THEN
   ASM_REWRITE_TAC[HD, TL, POLY_DIFF_AUX_ADD]);
 
 val POLY_DIFF_CMUL = store_thm("POLY_DIFF_CMUL",
  (Term`!p c. poly (diff (c ## p)) = poly (c ## diff p)`),
-  LIST_INDUCT_TAC THEN REWRITE_TAC[poly_diff_def, poly_cmul] THEN
+  LIST_INDUCT_TAC THEN REWRITE_TAC[poly_diff_def, poly_cmul_def] THEN
   REWRITE_TAC[NOT_CONS_NIL, HD, TL, POLY_DIFF_AUX_CMUL]);
 
 val POLY_DIFF_NEG = store_thm("POLY_DIFF_NEG",
@@ -422,36 +420,36 @@ val POLY_DIFF_MUL_LEMMA = store_thm("POLY_DIFF_MUL_LEMMA",
  (Term`!t h. poly (diff (CONS h t)) =
          poly (CONS (&0) (diff t) + t)`),
   REWRITE_TAC[poly_diff_def, NOT_CONS_NIL] THEN
-  LIST_INDUCT_TAC THEN REWRITE_TAC[poly_diff_aux, NOT_CONS_NIL, HD, TL] THENL
-   [REWRITE_TAC[FUN_EQ_THM, poly, poly_add, REAL_MUL_RZERO, REAL_ADD_LID],
-    REWRITE_TAC[FUN_EQ_THM, poly, POLY_DIFF_AUX_MUL_LEMMA, POLY_ADD] THEN
+  LIST_INDUCT_TAC THEN REWRITE_TAC[poly_diff_aux_def, NOT_CONS_NIL, HD, TL] THENL
+   [REWRITE_TAC[FUN_EQ_THM, poly_def, poly_add_def, REAL_MUL_RZERO, REAL_ADD_LID],
+    REWRITE_TAC[FUN_EQ_THM, poly_def, POLY_DIFF_AUX_MUL_LEMMA, POLY_ADD] THEN
     REAL_ARITH_TAC]);
 
 val POLY_DIFF_MUL = store_thm("POLY_DIFF_MUL",
  (Term`!p1 p2. poly (diff (p1 * p2)) =
            poly (p1 * diff p2 + diff p1 * p2)`),
-  LIST_INDUCT_TAC THEN REWRITE_TAC[poly_mul] THENL
-   [REWRITE_TAC[poly_diff_def, poly_add, poly_mul], ALL_TAC] THEN
+  LIST_INDUCT_TAC THEN REWRITE_TAC[poly_mul_def] THENL
+   [REWRITE_TAC[poly_diff_def, poly_add_def, poly_mul_def], ALL_TAC] THEN
   GEN_TAC THEN COND_CASES_TAC THEN ASM_REWRITE_TAC[] THENL
    [REWRITE_TAC[POLY_DIFF_CLAUSES] THEN
-    REWRITE_TAC[poly_add, poly_mul, POLY_ADD_RZERO, POLY_DIFF_CMUL],
+    REWRITE_TAC[poly_add_def, poly_mul_def, POLY_ADD_RZERO, POLY_DIFF_CMUL],
     ALL_TAC] THEN
   REWRITE_TAC[FUN_EQ_THM, POLY_DIFF_ADD, POLY_ADD] THEN
-  REWRITE_TAC[poly, POLY_ADD, POLY_DIFF_MUL_LEMMA, POLY_MUL] THEN
+  REWRITE_TAC[poly_def, POLY_ADD, POLY_DIFF_MUL_LEMMA, POLY_MUL] THEN
   ASM_REWRITE_TAC[POLY_DIFF_CMUL, POLY_ADD, POLY_MUL] THEN
   REAL_ARITH_TAC);
 
 val POLY_DIFF_EXP = store_thm("POLY_DIFF_EXP",
  (Term`!p n. poly (diff (p poly_exp (SUC n))) =
          poly (&(SUC n) ## (p poly_exp n) * diff p)`),
-  GEN_TAC THEN INDUCT_TAC THEN ONCE_REWRITE_TAC[poly_exp] THENL
-   [REWRITE_TAC[poly_exp, POLY_DIFF_MUL] THEN
+  GEN_TAC THEN INDUCT_TAC THEN ONCE_REWRITE_TAC[poly_exp_def] THENL
+   [REWRITE_TAC[poly_exp_def, POLY_DIFF_MUL] THEN
     REWRITE_TAC[FUN_EQ_THM, POLY_MUL, POLY_ADD, POLY_CMUL] THEN
-    REWRITE_TAC[poly, POLY_DIFF_CLAUSES, ADD1, ADD_CLAUSES] THEN
+    REWRITE_TAC[poly_def, POLY_DIFF_CLAUSES, ADD1, ADD_CLAUSES] THEN
     REAL_ARITH_TAC,
     REWRITE_TAC[POLY_DIFF_MUL] THEN
     ASM_REWRITE_TAC[POLY_MUL, POLY_ADD, FUN_EQ_THM, POLY_CMUL] THEN
-    REWRITE_TAC[poly_exp, POLY_MUL] THEN
+    REWRITE_TAC[poly_exp_def, POLY_MUL] THEN
     REWRITE_TAC[ADD1, GSYM REAL_OF_NUM_ADD] THEN
     REAL_ARITH_TAC]);
 
@@ -460,8 +458,8 @@ val POLY_DIFF_EXP_PRIME = store_thm("POLY_DIFF_EXP_PRIME",
          poly (&(SUC n) ## ([~a; &1] poly_exp n))`),
   REPEAT GEN_TAC THEN SIMP_TAC real_ac_ss [POLY_DIFF_EXP] THEN
   SIMP_TAC real_ac_ss [FUN_EQ_THM, POLY_CMUL, POLY_MUL] THEN
-  SIMP_TAC real_ac_ss [poly_diff_def, poly_diff_aux, TL, NOT_CONS_NIL] THEN
-  SIMP_TAC real_ac_ss [poly] THEN REAL_ARITH_TAC);
+  SIMP_TAC real_ac_ss [poly_diff_def, poly_diff_aux_def, TL, NOT_CONS_NIL] THEN
+  SIMP_TAC real_ac_ss [poly_def] THEN REAL_ARITH_TAC);
 
 (* ------------------------------------------------------------------------- *)
 (* Key property that f(a) = 0 ==> (x - a) divides p(x). Very delicate!       *)
@@ -472,41 +470,41 @@ val POLY_LINEAR_REM = store_thm("POLY_LINEAR_REM",
   LIST_INDUCT_TAC THEN REWRITE_TAC[] THENL
    [GEN_TAC THEN EXISTS_TAC (Term`[]:real list`) THEN
     EXISTS_TAC (Term`h:real`) THEN
-    REWRITE_TAC[poly_add, poly_mul, poly_cmul, NOT_CONS_NIL] THEN
+    REWRITE_TAC[poly_add_def, poly_mul_def, poly_cmul_def, NOT_CONS_NIL] THEN
     REWRITE_TAC[HD, TL, REAL_ADD_RID],
     X_GEN_TAC (Term`k:real`) THEN
     POP_ASSUM(STRIP_ASSUME_TAC o SPEC (Term`h:real`)) THEN
     EXISTS_TAC (Term`CONS (r:real) q`) THEN
     EXISTS_TAC (Term`r * a + k:real`) THEN
-    ASM_REWRITE_TAC[POLY_ADD_CLAUSES, POLY_MUL_CLAUSES, poly_cmul] THEN
+    ASM_REWRITE_TAC[POLY_ADD_CLAUSES, POLY_MUL_CLAUSES, poly_cmul_def] THEN
     REWRITE_TAC[CONS_11] THEN CONJ_TAC THENL
      [REAL_ARITH_TAC, ALL_TAC] THEN
     SPEC_TAC((Term`q:real list`),(Term`q:real list`)) THEN
     LIST_INDUCT_TAC THEN
-    REWRITE_TAC[POLY_ADD_CLAUSES, POLY_MUL_CLAUSES, poly_cmul] THEN
+    REWRITE_TAC[POLY_ADD_CLAUSES, POLY_MUL_CLAUSES, poly_cmul_def] THEN
     REWRITE_TAC[REAL_ADD_RID, REAL_MUL_LID] THEN
     SIMP_TAC real_ac_ss []]);
 
 val POLY_LINEAR_DIVIDES = store_thm("POLY_LINEAR_DIVIDES",
  (Term`!a p. (poly p a = &0) = (p = []) \/ ?q. p = [~a; &1] * q`),
   GEN_TAC THEN LIST_INDUCT_TAC THENL
-   [REWRITE_TAC[poly], ALL_TAC] THEN
+   [REWRITE_TAC[poly_def], ALL_TAC] THEN
   EQ_TAC THEN STRIP_TAC THENL
    [DISJ2_TAC THEN STRIP_ASSUME_TAC(SPEC_ALL POLY_LINEAR_REM) THEN
     EXISTS_TAC (Term`q:real list`) THEN ASM_REWRITE_TAC[] THEN
     SUBGOAL_THEN (Term`r = &0`) SUBST_ALL_TAC THENL
      [UNDISCH_TAC (Term`poly (CONS h t) a = &0`) THEN
       ASM_REWRITE_TAC[] THEN REWRITE_TAC[POLY_ADD, POLY_MUL] THEN
-      REWRITE_TAC[poly, REAL_MUL_RZERO, REAL_ADD_RID, REAL_MUL_RID] THEN
+      REWRITE_TAC[poly_def, REAL_MUL_RZERO, REAL_ADD_RID, REAL_MUL_RID] THEN
       REWRITE_TAC[REAL_ARITH (Term`~a + a = &0`)] THEN REAL_ARITH_TAC,
-      REWRITE_TAC[poly_mul] THEN REWRITE_TAC[NOT_CONS_NIL] THEN
+      REWRITE_TAC[poly_mul_def] THEN REWRITE_TAC[NOT_CONS_NIL] THEN
       SPEC_TAC((Term`q:real list`),(Term`q:real list`)) THEN LIST_INDUCT_TAC THENL
-       [REWRITE_TAC[poly_cmul, poly_add, NOT_CONS_NIL, HD, TL, REAL_ADD_LID],
-        REWRITE_TAC[poly_cmul, poly_add, NOT_CONS_NIL, HD, TL, REAL_ADD_LID]]],
-    ASM_REWRITE_TAC[] THEN REWRITE_TAC[poly],
-    ASM_REWRITE_TAC[] THEN REWRITE_TAC[poly] THEN
-    REWRITE_TAC[POLY_MUL] THEN REWRITE_TAC[poly] THEN
-    REWRITE_TAC[poly, REAL_MUL_RZERO, REAL_ADD_RID, REAL_MUL_RID] THEN
+       [REWRITE_TAC[poly_cmul_def, poly_add_def, NOT_CONS_NIL, HD, TL, REAL_ADD_LID],
+        REWRITE_TAC[poly_cmul_def, poly_add_def, NOT_CONS_NIL, HD, TL, REAL_ADD_LID]]],
+    ASM_REWRITE_TAC[] THEN REWRITE_TAC[poly_def],
+    ASM_REWRITE_TAC[] THEN REWRITE_TAC[poly_def] THEN
+    REWRITE_TAC[POLY_MUL] THEN REWRITE_TAC[poly_def] THEN
+    REWRITE_TAC[poly_def, REAL_MUL_RZERO, REAL_ADD_RID, REAL_MUL_RID] THEN
     REWRITE_TAC[REAL_ARITH (Term`~a + a = &0`)] THEN REAL_ARITH_TAC]);
 
 (* ------------------------------------------------------------------------- *)
@@ -519,9 +517,9 @@ val POLY_LENGTH_MUL = store_thm("POLY_LENGTH_MUL",
     val lemma = prove
    ((Term`!p h k a. LENGTH (k ## p + CONS h (a ## p)) = SUC(LENGTH p)`),
     LIST_INDUCT_TAC THEN
-    ASM_REWRITE_TAC[poly_cmul, POLY_ADD_CLAUSES, LENGTH])
+    ASM_REWRITE_TAC[poly_cmul_def, POLY_ADD_CLAUSES, LENGTH])
   in
-    REWRITE_TAC[poly_mul, NOT_CONS_NIL, lemma]
+    REWRITE_TAC[poly_mul_def, NOT_CONS_NIL, lemma]
   end);
 
 (* ------------------------------------------------------------------------- *)
@@ -542,7 +540,7 @@ val POLY_ROOTS_INDEX_LEMMA = store_thm("POLY_ROOTS_INDEX_LEMMA",
       UNDISCH_TAC (Term`~(poly ([~a; &1] * q) = poly [])`) THEN
       POP_ASSUM MP_TAC THEN REWRITE_TAC[POLY_LENGTH_MUL, SUC_INJ] THEN
       DISCH_TAC THEN ASM_CASES_TAC (Term`poly q = poly []`) THENL
-       [ASM_REWRITE_TAC[POLY_MUL, poly, REAL_MUL_RZERO, FUN_EQ_THM],
+       [ASM_REWRITE_TAC[POLY_MUL, poly_def, REAL_MUL_RZERO, FUN_EQ_THM],
         DISCH_THEN(K ALL_TAC)] THEN
       DISCH_THEN(MP_TAC o SPEC (Term`q:real list`)) THEN ASM_REWRITE_TAC[] THEN
       DISCH_THEN(X_CHOOSE_TAC (Term`i:num->real`)) THEN
@@ -550,7 +548,7 @@ val POLY_ROOTS_INDEX_LEMMA = store_thm("POLY_ROOTS_INDEX_LEMMA",
       REWRITE_TAC[POLY_MUL, LE, REAL_ENTIRE] THEN
       X_GEN_TAC (Term`x:real`) THEN DISCH_THEN(DISJ_CASES_THEN MP_TAC) THENL
        [DISCH_THEN(fn th => EXISTS_TAC (Term`SUC n`) THEN MP_TAC th) THEN
-        SIMP_TAC real_ac_ss [] THEN REWRITE_TAC[poly] THEN REAL_ARITH_TAC,
+        SIMP_TAC real_ac_ss [] THEN REWRITE_TAC[poly_def] THEN REAL_ARITH_TAC,
         DISCH_THEN(ANTE_RES_THEN MP_TAC) THEN
         DISCH_THEN(X_CHOOSE_THEN (Term`m:num`) STRIP_ASSUME_TAC) THEN
         EXISTS_TAC (Term`m:num`) THEN ASM_SIMP_TAC real_ac_ss [] THEN
@@ -588,7 +586,7 @@ val POLY_ROOTS_FINITE = store_thm("POLY_ROOTS_FINITE",
  (Term`!p. ~(poly p = poly []) =
        ?N i. !x. (poly p(x) = &0) ==> ?n:num. n < N /\ (x = i n)`),
   GEN_TAC THEN EQ_TAC THEN REWRITE_TAC[POLY_ROOTS_FINITE_LEMMA] THEN
-  REWRITE_TAC[FUN_EQ_THM, LEFT_IMP_EXISTS_THM, NOT_FORALL_THM, poly] THEN
+  REWRITE_TAC[FUN_EQ_THM, LEFT_IMP_EXISTS_THM, NOT_FORALL_THM, poly_def] THEN
   MP_TAC(GENL [(Term`i:num->real`), (Term`N:num`)]
    (SPECL [(Term`i:num->real`), (Term`N:num`), (Term`\x. poly p x = &0`)] FINITE_LEMMA)) THEN
   REWRITE_TAC[] THEN MESON_TAC[REAL_LT_REFL]);
@@ -616,7 +614,7 @@ val POLY_ENTIRE = store_thm("POLY_ENTIRE",
   REPEAT GEN_TAC THEN EQ_TAC THENL
    [MESON_TAC[POLY_ENTIRE_LEMMA],
     REWRITE_TAC[FUN_EQ_THM, POLY_MUL] THEN
-    STRIP_TAC THEN ASM_REWRITE_TAC[REAL_MUL_RZERO, REAL_MUL_LZERO, poly]]);
+    STRIP_TAC THEN ASM_REWRITE_TAC[REAL_MUL_RZERO, REAL_MUL_LZERO, poly_def]]);
 
 val POLY_MUL_LCANCEL = store_thm("POLY_MUL_LCANCEL",
  (Term`!p q r. (poly (p * q) = poly (p * r)) =
@@ -624,7 +622,7 @@ val POLY_MUL_LCANCEL = store_thm("POLY_MUL_LCANCEL",
   let
     val lemma1 = prove
      ((Term`!p q. (poly (p + poly_neg q) = poly []) = (poly p = poly q)`),
-      REWRITE_TAC[FUN_EQ_THM, POLY_ADD, POLY_NEG, poly] THEN
+      REWRITE_TAC[FUN_EQ_THM, POLY_ADD, POLY_NEG, poly_def] THEN
       REWRITE_TAC[REAL_ARITH (Term`(p + ~q = &0) = (p = q)`)])
     val lemma2 = prove
      ((Term`!p q r. poly (p * q + poly_neg(p * r)) = poly (p * (q + poly_neg(r)))`),
@@ -638,17 +636,17 @@ val POLY_MUL_LCANCEL = store_thm("POLY_MUL_LCANCEL",
 
 val POLY_EXP_EQ_0 = store_thm("POLY_EXP_EQ_0",
  (Term`!p n. (poly (p poly_exp n) = poly []) = (poly p = poly []) /\ ~(n = 0)`),
-  REPEAT GEN_TAC THEN REWRITE_TAC[FUN_EQ_THM, poly] THEN
+  REPEAT GEN_TAC THEN REWRITE_TAC[FUN_EQ_THM, poly_def] THEN
   REWRITE_TAC [LEFT_AND_FORALL_THM] THEN AP_TERM_TAC THEN ABS_TAC THEN
   SPEC_TAC((Term`n:num`),(Term`n:num`)) THEN INDUCT_TAC THEN
-  SIMP_TAC real_ac_ss [poly_exp, poly, REAL_MUL_RZERO, REAL_ADD_RID,
+  SIMP_TAC real_ac_ss [poly_exp_def, poly_def, REAL_MUL_RZERO, REAL_ADD_RID,
     REAL_OF_NUM_EQ, NOT_SUC] THEN
-  ASM_REWRITE_TAC[POLY_MUL, poly, REAL_ENTIRE] THEN
+  ASM_REWRITE_TAC[POLY_MUL, poly_def, REAL_ENTIRE] THEN
   MESON_TAC []);
 
 val POLY_PRIME_EQ_0 = store_thm("POLY_PRIME_EQ_0",
  (Term`!a. ~(poly [a; &1] = poly [])`),
-  GEN_TAC THEN REWRITE_TAC[FUN_EQ_THM, poly] THEN
+  GEN_TAC THEN REWRITE_TAC[FUN_EQ_THM, poly_def] THEN
   DISCH_THEN(MP_TAC o SPEC (Term`&1 - a`)) THEN
   REAL_ARITH_TAC);
 
@@ -663,10 +661,10 @@ val POLY_EXP_PRIME_EQ_0 = store_thm("POLY_EXP_PRIME_EQ_0",
 val POLY_ZERO_LEMMA = store_thm("POLY_ZERO_LEMMA",
  (Term`!h t. (poly (CONS h t) = poly []) ==> (h = &0) /\ (poly t = poly [])`),
   let
-    val lemma = REWRITE_RULE[FUN_EQ_THM, poly] POLY_ROOTS_FINITE
+    val lemma = REWRITE_RULE[FUN_EQ_THM, poly_def] POLY_ROOTS_FINITE
   in
     REPEAT GEN_TAC
-    THEN SIMP_TAC real_ac_ss [FUN_EQ_THM, poly]
+    THEN SIMP_TAC real_ac_ss [FUN_EQ_THM, poly_def]
     THEN ASM_CASES_TAC (Term`h = &0`)
     THEN ASM_SIMP_TAC real_ac_ss []
     THENL [
@@ -692,7 +690,7 @@ val POLY_ZERO = store_thm("POLY_ZERO",
   LIST_INDUCT_TAC THEN ASM_REWRITE_TAC[FORALL] THEN EQ_TAC THENL
    [DISCH_THEN(MP_TAC o MATCH_MP POLY_ZERO_LEMMA) THEN ASM_REWRITE_TAC[],
     POP_ASSUM(SUBST1_TAC o SYM) THEN STRIP_TAC THEN
-    ASM_REWRITE_TAC[FUN_EQ_THM, poly] THEN REAL_ARITH_TAC]);
+    ASM_REWRITE_TAC[FUN_EQ_THM, poly_def] THEN REAL_ARITH_TAC]);
 
 (* ------------------------------------------------------------------------- *)
 (* Useful triviality.                                                        *)
@@ -702,17 +700,17 @@ val POLY_DIFF_AUX_ISZERO = store_thm("POLY_DIFF_AUX_ISZERO",
  (Term`!p n. EVERY (\c. c = &0) (poly_diff_aux (SUC n) p) =
          EVERY (\c. c = &0) p`),
   LIST_INDUCT_TAC THEN ASM_REWRITE_TAC
-   [FORALL, poly_diff_aux, REAL_ENTIRE, REAL_OF_NUM_EQ, NOT_SUC]);
+   [FORALL, poly_diff_aux_def, REAL_ENTIRE, REAL_OF_NUM_EQ, NOT_SUC]);
 
 
 val POLY_DIFF_ISZERO = store_thm("POLY_DIFF_ISZERO",
  (Term`!p. (poly (diff p) = poly []) ==> ?h. poly p = poly [h]`),
   REWRITE_TAC[POLY_ZERO] THEN
   LIST_INDUCT_TAC THEN ASM_REWRITE_TAC[POLY_DIFF_CLAUSES, FORALL] THENL
-   [EXISTS_TAC (Term`&0`) THEN REWRITE_TAC[FUN_EQ_THM, poly] THEN REAL_ARITH_TAC,
+   [EXISTS_TAC (Term`&0`) THEN REWRITE_TAC[FUN_EQ_THM, poly_def] THEN REAL_ARITH_TAC,
     REWRITE_TAC[ONE, POLY_DIFF_AUX_ISZERO] THEN
     REWRITE_TAC[GSYM POLY_ZERO] THEN DISCH_TAC THEN
-    EXISTS_TAC (Term`h:real`) THEN ASM_REWRITE_TAC[poly, FUN_EQ_THM]]);
+    EXISTS_TAC (Term`h:real`) THEN ASM_REWRITE_TAC[poly_def, FUN_EQ_THM]]);
 
 val POLY_DIFF_ZERO = store_thm("POLY_DIFF_ZERO",
  (Term`!p. (poly p = poly []) ==> (poly (diff p) = poly [])`),
@@ -722,7 +720,7 @@ val POLY_DIFF_ZERO = store_thm("POLY_DIFF_ZERO",
   DISCH_THEN(CONJUNCTS_THEN2 ASSUME_TAC MP_TAC) THEN
   SPEC_TAC((Term`1:num`),(Term`n:num`)) THEN POP_ASSUM_LIST(K ALL_TAC) THEN
   SPEC_TAC((Term`t:real list`),(Term`t:real list`)) THEN
-  LIST_INDUCT_TAC THEN REWRITE_TAC[FORALL, poly_diff_aux] THEN
+  LIST_INDUCT_TAC THEN REWRITE_TAC[FORALL, poly_diff_aux_def] THEN
   REPEAT STRIP_TAC THEN ASM_REWRITE_TAC[REAL_MUL_RZERO] THEN
   FIRST_ASSUM MATCH_MP_TAC THEN ASM_REWRITE_TAC[]);
 
@@ -730,7 +728,7 @@ val POLY_DIFF_WELLDEF = store_thm("POLY_DIFF_WELLDEF",
  (Term`!p q. (poly p = poly q) ==> (poly (diff p) = poly (diff q))`),
   REPEAT STRIP_TAC THEN MP_TAC(SPEC (Term`p + poly_neg(q)`) POLY_DIFF_ZERO) THEN
   REWRITE_TAC[FUN_EQ_THM, POLY_DIFF_ADD, POLY_DIFF_NEG, POLY_ADD] THEN
-  ASM_REWRITE_TAC[POLY_NEG, poly, REAL_ARITH (Term`a + ~a = &0`)] THEN
+  ASM_REWRITE_TAC[POLY_NEG, poly_def, REAL_ARITH (Term`a + ~a = &0`)] THEN
   REWRITE_TAC[REAL_ARITH (Term`(a + ~b = &0) = (a = b)`)]);
 
 (* ------------------------------------------------------------------------- *)
@@ -744,7 +742,7 @@ val POLY_PRIMES = store_thm("POLY_PRIMES",
  (Term`!a p q. [a; &1] poly_divides (p * q)
                            =
                [a; &1] poly_divides p \/ [a; &1] poly_divides q`),
- REPEAT GEN_TAC THEN REWRITE_TAC[poly_divides, POLY_MUL, FUN_EQ_THM, poly] THEN
+ REPEAT GEN_TAC THEN REWRITE_TAC[poly_divides, POLY_MUL, FUN_EQ_THM, poly_def] THEN
  REWRITE_TAC[REAL_MUL_RZERO, REAL_ADD_RID, REAL_MUL_RID] THEN EQ_TAC THENL
  [DISCH_THEN(X_CHOOSE_THEN (Term`r:real list`)
   (MP_TAC o SPEC (Term`~a:real`))) THEN
@@ -754,9 +752,9 @@ val POLY_PRIMES = store_thm("POLY_PRIMES",
      REWRITE_TAC[REAL_NEG_NEG] THEN
      DISCH_THEN(DISJ_CASES_THEN2 SUBST_ALL_TAC
         (X_CHOOSE_THEN (Term`s:real list`) SUBST_ALL_TAC)) THENL
-      [EXISTS_TAC (Term`[]:real list`) THEN REWRITE_TAC[poly, REAL_MUL_RZERO],
+      [EXISTS_TAC (Term`[]:real list`) THEN REWRITE_TAC[poly_def, REAL_MUL_RZERO],
        EXISTS_TAC (Term`s:real list`) THEN GEN_TAC THEN
-       REWRITE_TAC[POLY_MUL, poly] THEN REAL_ARITH_TAC]),
+       REWRITE_TAC[POLY_MUL, poly_def] THEN REAL_ARITH_TAC]),
     DISCH_THEN(DISJ_CASES_THEN(X_CHOOSE_TAC (Term`s:real list`))) THEN
     ASM_REWRITE_TAC[] THENL
      [EXISTS_TAC (Term`s * q`), EXISTS_TAC (Term`p * s`)] THEN
@@ -765,7 +763,7 @@ val POLY_PRIMES = store_thm("POLY_PRIMES",
 val POLY_DIVIDES_REFL = store_thm("POLY_DIVIDES_REFL",
  (Term`!p. p poly_divides p`),
   GEN_TAC THEN REWRITE_TAC[poly_divides] THEN EXISTS_TAC (Term`[&1]`) THEN
-  REWRITE_TAC[FUN_EQ_THM, POLY_MUL, poly] THEN REAL_ARITH_TAC);
+  REWRITE_TAC[FUN_EQ_THM, POLY_MUL, poly_def] THEN REAL_ARITH_TAC);
 
 val POLY_DIVIDES_TRANS = store_thm("POLY_DIVIDES_TRANS",
  (Term`!p q r. p poly_divides q /\ q poly_divides r ==> p poly_divides r`),
@@ -785,7 +783,7 @@ val POLY_DIVIDES_EXP = store_thm("POLY_DIVIDES_EXP",
   MATCH_MP_TAC POLY_DIVIDES_TRANS THEN
   EXISTS_TAC (Term`p poly_exp (m + d)`) THEN ASM_REWRITE_TAC[] THEN
   REWRITE_TAC[poly_divides] THEN EXISTS_TAC (Term`p:real list`) THEN
-  REWRITE_TAC[poly_exp, FUN_EQ_THM, POLY_MUL] THEN
+  REWRITE_TAC[poly_exp_def, FUN_EQ_THM, POLY_MUL] THEN
   REAL_ARITH_TAC);
 
 val POLY_EXP_DIVIDES = store_thm("POLY_EXP_DIVIDES",
@@ -831,7 +829,7 @@ val POLY_DIVIDES_ZERO = store_thm("POLY_DIVIDES_ZERO",
  (Term`!p q. (poly p = poly []) ==> q poly_divides p`),
   REPEAT GEN_TAC THEN DISCH_TAC THEN REWRITE_TAC[poly_divides] THEN
   EXISTS_TAC (Term`[]:real list`) THEN
-  ASM_REWRITE_TAC[FUN_EQ_THM, POLY_MUL, poly, REAL_MUL_RZERO]);
+  ASM_REWRITE_TAC[FUN_EQ_THM, POLY_MUL, poly_def, REAL_MUL_RZERO]);
 
 (* ------------------------------------------------------------------------- *)
 (* At last, we can consider the order of a root.                             *)
@@ -893,7 +891,7 @@ val POLY_ORDER_EXISTS = store_thm("POLY_ORDER_EXISTS",
       EXISTS_TAC (Term`s:real list`)
       THEN SPEC_TAC((Term`n:num`),(Term`n:num`))
       THEN INDUCT_TAC
-      THEN ASM_REWRITE_TAC[poly_exp, FUN_EQ_THM, POLY_MUL, poly]
+      THEN ASM_REWRITE_TAC[poly_exp_def, FUN_EQ_THM, POLY_MUL, poly_def]
       THEN REAL_ARITH_TAC,
       DISCH_THEN(X_CHOOSE_THEN (Term`r:real list`) MP_TAC)
       THEN SPEC_TAC((Term`n:num`),(Term`n:num`))
@@ -904,18 +902,18 @@ val POLY_ORDER_EXISTS = store_thm("POLY_ORDER_EXISTS",
         THEN CONV_TAC CONTRAPOS_CONV
         THEN REWRITE_TAC[]
         THEN DISCH_THEN SUBST1_TAC
-        THEN REWRITE_TAC[poly, poly_exp, POLY_MUL]
+        THEN REWRITE_TAC[poly_def, poly_exp_def, POLY_MUL]
         THEN REAL_ARITH_TAC,
         REWRITE_TAC[]
         THEN ONCE_ASM_REWRITE_TAC[]
-        THEN ONCE_REWRITE_TAC[poly_exp]
+        THEN ONCE_REWRITE_TAC[poly_exp_def]
         THEN REWRITE_TAC[GSYM POLY_MUL_ASSOC, POLY_MUL_LCANCEL]
         THEN REWRITE_TAC[DE_MORGAN_THM]
         THEN CONJ_TAC
         THENL [
           REWRITE_TAC[FUN_EQ_THM]
           THEN DISCH_THEN(MP_TAC o SPEC (Term`a + &1`))
-          THEN REWRITE_TAC[poly]
+          THEN REWRITE_TAC[poly_def]
           THEN REAL_ARITH_TAC,
           DISCH_THEN(ANTE_RES_THEN MP_TAC)
           THEN REWRITE_TAC[]
@@ -949,7 +947,7 @@ val ORDER = store_thm("ORDER",
      [FIRST_ASSUM(UNDISCH_TAC o assert is_neg o concl) THEN
       CONV_TAC CONTRAPOS_CONV THEN REWRITE_TAC[poly_divides] THEN
       DISCH_THEN SUBST1_TAC THEN EXISTS_TAC (Term`[]:real list`) THEN
-      REWRITE_TAC[FUN_EQ_THM, POLY_MUL, poly, REAL_MUL_RZERO],
+      REWRITE_TAC[FUN_EQ_THM, POLY_MUL, poly_def, REAL_MUL_RZERO],
       ASM_REWRITE_TAC[] THEN CONV_TAC SYM_CONV THEN
       MATCH_MP_TAC SELECT_UNIQUE THEN REWRITE_TAC[]],
     ONCE_ASM_REWRITE_TAC[] THEN CONV_TAC SELECT_CONV] THEN
@@ -976,23 +974,23 @@ val ORDER_POLY = store_thm("ORDER_POLY",
 val ORDER_ROOT = store_thm("ORDER_ROOT",
  (Term`!p a. (poly p a = &0) = (poly p = poly []) \/ ~(poly_order a p = 0)`),
   REPEAT GEN_TAC THEN ASM_CASES_TAC (Term`poly p = poly []`) THEN
-  ASM_REWRITE_TAC[poly] THEN EQ_TAC THENL
+  ASM_REWRITE_TAC[poly_def] THEN EQ_TAC THENL
    [DISCH_THEN(MP_TAC o REWRITE_RULE[POLY_LINEAR_DIVIDES]) THEN
     ASM_CASES_TAC (Term`p:real list = []`) THENL [ASM_MESON_TAC[], ALL_TAC] THEN
     ASM_REWRITE_TAC[] THEN
     DISCH_THEN(X_CHOOSE_THEN (Term`q:real list`) SUBST_ALL_TAC) THEN DISCH_TAC THEN
     FIRST_ASSUM(MP_TAC o SPEC (Term`a:real`) o MATCH_MP ORDER_THM) THEN
-    ASM_REWRITE_TAC[poly_exp, DE_MORGAN_THM] THEN DISJ2_TAC THEN
+    ASM_REWRITE_TAC[poly_exp_def, DE_MORGAN_THM] THEN DISJ2_TAC THEN
     REWRITE_TAC[poly_divides] THEN EXISTS_TAC (Term`q:real list`) THEN
-    REWRITE_TAC[FUN_EQ_THM, POLY_MUL, poly] THEN REAL_ARITH_TAC,
+    REWRITE_TAC[FUN_EQ_THM, POLY_MUL, poly_def] THEN REAL_ARITH_TAC,
     DISCH_TAC THEN
     FIRST_ASSUM(MP_TAC o SPEC (Term`a:real`) o MATCH_MP ORDER_THM) THEN
     UNDISCH_TAC (Term`~(poly_order a p = 0)`) THEN
     SPEC_TAC((Term`poly_order a p`),(Term`n:num`)) THEN
-    INDUCT_TAC THEN ASM_REWRITE_TAC[poly_exp, NOT_SUC] THEN
+    INDUCT_TAC THEN ASM_REWRITE_TAC[poly_exp_def, NOT_SUC] THEN
     DISCH_THEN(MP_TAC o CONJUNCT1) THEN REWRITE_TAC[poly_divides] THEN
     DISCH_THEN(X_CHOOSE_THEN (Term`s:real list`) SUBST1_TAC) THEN
-    REWRITE_TAC[POLY_MUL, poly] THEN REAL_ARITH_TAC]);
+    REWRITE_TAC[POLY_MUL, poly_def] THEN REAL_ARITH_TAC]);
 
 val ORDER_DIVIDES = store_thm("ORDER_DIVIDES",
  (Term`!p a n. ([~a; &1] poly_exp n) poly_divides p =
@@ -1000,7 +998,7 @@ val ORDER_DIVIDES = store_thm("ORDER_DIVIDES",
   REPEAT GEN_TAC THEN ASM_CASES_TAC (Term`poly p = poly []`) THEN
   ASM_REWRITE_TAC[] THENL
    [ASM_REWRITE_TAC[poly_divides] THEN EXISTS_TAC (Term`[]:real list`) THEN
-    REWRITE_TAC[FUN_EQ_THM, POLY_MUL, poly, REAL_MUL_RZERO],
+    REWRITE_TAC[FUN_EQ_THM, POLY_MUL, poly_def, REAL_MUL_RZERO],
     ASM_MESON_TAC[ORDER_THM, POLY_EXP_DIVIDES, NOT_LE, LE_SUC_LT]]);
 
 val ORDER_DECOMP = store_thm("ORDER_DECOMP",
@@ -1015,7 +1013,7 @@ val ORDER_DECOMP = store_thm("ORDER_DECOMP",
   UNDISCH_TAC (Term`~([~ a; &1] poly_exp SUC (poly_order a p) poly_divides p)`) THEN
   ASM_REWRITE_TAC[] THEN REWRITE_TAC[poly_divides] THEN
   EXISTS_TAC (Term`r:real list`) THEN
-  ASM_REWRITE_TAC[POLY_MUL, FUN_EQ_THM, poly_exp] THEN
+  ASM_REWRITE_TAC[POLY_MUL, FUN_EQ_THM, poly_exp_def] THEN
   REAL_ARITH_TAC);
 
 (* ------------------------------------------------------------------------- *)
@@ -1052,7 +1050,7 @@ val ORDER_MUL = store_thm("ORDER_MUL",
     (SPEC (Term`a:real`) (MATCH_MP ORDER_DECOMP (ASSUME (Term`~(poly p = poly [])`))))
     THEN X_CHOOSE_THEN (Term`s: real list`) STRIP_ASSUME_TAC
     (SPEC (Term`a:real`) (MATCH_MP ORDER_DECOMP (ASSUME (Term`~(poly q = poly [])`))))
-    THEN ASM_REWRITE_TAC[poly_divides, FUN_EQ_THM, POLY_EXP_ADD, POLY_MUL, poly_exp]
+    THEN ASM_REWRITE_TAC[poly_divides, FUN_EQ_THM, POLY_EXP_ADD, POLY_MUL, poly_exp_def]
     THEN DISCH_THEN(X_CHOOSE_THEN (Term`t:real list`) STRIP_ASSUME_TAC)
     THEN SUBGOAL_THEN (Term`[~a; &1] poly_divides (r * s)`) MP_TAC
     THENL [
@@ -1106,7 +1104,7 @@ val ORDER_DIFF = store_thm("ORDER_DIFF",
     EXISTS_TAC (Term`[~a; &1] * (diff q) + &(SUC n) ## q`) THEN
     REWRITE_TAC[POLY_DIFF_MUL, POLY_DIFF_EXP_PRIME,
       POLY_ADD, POLY_MUL, POLY_CMUL] THEN
-    REWRITE_TAC[poly_exp, POLY_MUL] THEN REAL_ARITH_TAC,
+    REWRITE_TAC[poly_exp_def, POLY_MUL] THEN REAL_ARITH_TAC,
     REWRITE_TAC[FUN_EQ_THM, poly_divides, POLY_DIFF_MUL, POLY_DIFF_EXP_PRIME,
       POLY_ADD, POLY_MUL, POLY_CMUL] THEN
     DISCH_THEN(X_CHOOSE_THEN (Term`r:real list`) ASSUME_TAC) THEN
@@ -1138,7 +1136,7 @@ val ORDER_DIFF = store_thm("ORDER_DIFF",
        MATCH_MP_TAC REAL_MUL_RINV THEN
        REWRITE_TAC[REAL_OF_NUM_EQ, NOT_SUC], ALL_TAC] THEN
     FIRST_ASSUM(MP_TAC o SPEC (Term`x:real`)) THEN
-    REWRITE_TAC[poly_exp, POLY_MUL, POLY_ADD, POLY_NEG] THEN
+    REWRITE_TAC[poly_exp_def, POLY_MUL, POLY_ADD, POLY_NEG] THEN
     REAL_ARITH_TAC]);
 
 (* ------------------------------------------------------------------------- *)
@@ -1213,18 +1211,18 @@ val RSQUAREFREE_ROOTS = store_thm("RSQUAREFREE_ROOTS",
   GEN_TAC THEN REWRITE_TAC[rsquarefree] THEN
   ASM_CASES_TAC (Term`poly p = poly []`) THEN ASM_REWRITE_TAC[] THENL
    [FIRST_ASSUM(SUBST1_TAC o MATCH_MP POLY_DIFF_ZERO) THEN
-    ASM_REWRITE_TAC[poly, NOT_FORALL_THM],
+    ASM_REWRITE_TAC[poly_def, NOT_FORALL_THM],
     ASM_CASES_TAC (Term`poly(diff p) = poly []`) THEN ASM_REWRITE_TAC[] THENL
      [FIRST_ASSUM(X_CHOOSE_THEN (Term`h:real`) MP_TAC o
         MATCH_MP POLY_DIFF_ISZERO) THEN
       DISCH_THEN(fn th => ASSUME_TAC th THEN MP_TAC th) THEN
       DISCH_THEN(fn th => REWRITE_TAC[MATCH_MP ORDER_POLY th]) THEN
-      UNDISCH_TAC (Term`~(poly p = poly [])`) THEN ASM_REWRITE_TAC[poly] THEN
-      REWRITE_TAC[FUN_EQ_THM, poly, REAL_MUL_RZERO, REAL_ADD_RID] THEN
+      UNDISCH_TAC (Term`~(poly p = poly [])`) THEN ASM_REWRITE_TAC[poly_def] THEN
+      REWRITE_TAC[FUN_EQ_THM, poly_def, REAL_MUL_RZERO, REAL_ADD_RID] THEN
       DISCH_TAC THEN ASM_REWRITE_TAC[] THEN
       X_GEN_TAC (Term`a:real`) THEN DISJ1_TAC THEN
       MP_TAC(SPECL [(Term`[h:real]`), (Term`a:real`)] ORDER_ROOT) THEN
-      ASM_REWRITE_TAC[FUN_EQ_THM, poly, REAL_MUL_RZERO, REAL_ADD_RID],
+      ASM_REWRITE_TAC[FUN_EQ_THM, poly_def, REAL_MUL_RZERO, REAL_ADD_RID],
       ASM_REWRITE_TAC[ORDER_ROOT, DE_MORGAN_THM, ONE] THEN
       ASM_MESON_TAC[ORDER_DIFF, SUC_INJ]]]);
 
@@ -1243,15 +1241,15 @@ val RSQUAREFREE_DECOMP = store_thm("RSQUAREFREE_DECOMP",
    [REWRITE_TAC[FUN_EQ_THM, POLY_MUL] THEN GEN_TAC THEN
     AP_THM_TAC THEN AP_TERM_TAC THEN
     GEN_REWRITE_TAC (LAND_CONV o LAND_CONV o RAND_CONV) [ONE] THEN
-    REWRITE_TAC[poly_exp, POLY_MUL] THEN
-    REWRITE_TAC[poly] THEN REAL_ARITH_TAC,
+    REWRITE_TAC[poly_exp_def, POLY_MUL] THEN
+    REWRITE_TAC[poly_def] THEN REAL_ARITH_TAC,
     DISCH_TAC THEN UNDISCH_TAC (Term`~([~a; &1] poly_divides q)`) THEN
     REWRITE_TAC[poly_divides] THEN
     UNDISCH_TAC (Term`poly q a = &0`) THEN
     GEN_REWRITE_TAC LAND_CONV [POLY_LINEAR_DIVIDES] THEN
     ASM_CASES_TAC (Term`q:real list = []`) THEN ASM_REWRITE_TAC[] THENL
      [EXISTS_TAC (Term`[] : real list`) THEN REWRITE_TAC[FUN_EQ_THM] THEN
-      REWRITE_TAC[POLY_MUL, poly, REAL_MUL_RZERO],
+      REWRITE_TAC[POLY_MUL, poly_def, REAL_MUL_RZERO],
       MESON_TAC[]]]);
 
 val POLY_SQUAREFREE_DECOMP = store_thm("POLY_SQUAREFREE_DECOMP",
@@ -1281,19 +1279,20 @@ val POLY_SQUAREFREE_DECOMP = store_thm("POLY_SQUAREFREE_DECOMP",
 (* Normalization of a polynomial.                                            *)
 (* ------------------------------------------------------------------------- *)
 
-val normalize = new_recursive_definition list_Axiom "normalize"
-  (Term`(normalize [] = []) /\
-   (normalize (CONS h t) = (if (normalize t = []) then
-                              if (h = &0) then [] else [h]
-                            else CONS h (normalize t)))`);
+Definition normalize[nocompute]:
+  (normalize [] = []) /\
+  (normalize (CONS h t) = (if (normalize t = []) then
+                             if (h = &0) then [] else [h]
+                           else CONS h (normalize t)))
+End
 
 val POLY_NORMALIZE = store_thm("POLY_NORMALIZE",
  (Term`!p. poly (normalize p) = poly p`),
-  LIST_INDUCT_TAC THEN REWRITE_TAC[normalize, poly] THEN
+  LIST_INDUCT_TAC THEN REWRITE_TAC[normalize, poly_def] THEN
   ASM_CASES_TAC (Term`h = &0`) THEN ASM_REWRITE_TAC[] THEN
-  COND_CASES_TAC THEN ASM_REWRITE_TAC[poly, FUN_EQ_THM] THEN
+  COND_CASES_TAC THEN ASM_REWRITE_TAC[poly_def, FUN_EQ_THM] THEN
   UNDISCH_TAC (Term`poly (normalize t) = poly t`) THEN
-  DISCH_THEN(SUBST1_TAC o SYM) THEN ASM_REWRITE_TAC[poly] THEN
+  DISCH_THEN(SUBST1_TAC o SYM) THEN ASM_REWRITE_TAC[poly_def] THEN
   REWRITE_TAC[REAL_MUL_RZERO, REAL_ADD_LID]);
 
 (* ------------------------------------------------------------------------- *)
@@ -1352,7 +1351,7 @@ val POLY_MONO = store_thm("POLY_MONO",
  (Term`!x k p. abs(x) <= k ==> abs(poly p x) <= poly (MAP abs p) k`),
   GEN_TAC THEN GEN_TAC THEN REWRITE_TAC[RIGHT_FORALL_IMP_THM] THEN
   DISCH_TAC THEN LIST_INDUCT_TAC THEN
-  REWRITE_TAC[poly, REAL_LE_REFL, MAP, REAL_ABS_0] THEN
+  REWRITE_TAC[poly_def, REAL_LE_REFL, MAP, REAL_ABS_0] THEN
   MATCH_MP_TAC REAL_LE_TRANS THEN
   EXISTS_TAC (Term`abs(h) + abs(x * poly t x)`) THEN
   REWRITE_TAC[REAL_ABS_TRIANGLE, REAL_LE_LADD] THEN
